spot/GC.SPOT.HeapExpansion.fst
@@ -12,6 +12,7 @@ open GC.Gen.Promote
 module MH = GC.Spec.MajorHeap
 module SpecAlloc = GC.Spec.Allocator
 module SpecMajorAlloc = GC.Spec.MajorAllocator
+module SpecMajorAllocMultiAlloc = GC.Spec.MajorAllocator.MultiAlloc
 module CG = GC.Gen.CombinedGraph
 module GenInv = GC.Gen.HeapInvariant
 
@@ -287,6 +288,29 @@ let spot_chunked_major_alloc_shape_active_head_split
            r.major_alloc_out r.major_fp_out fuel))
   = GenInv.chunked_major_alloc_shape_active_head_split
       mh fp requested_wz fuel
+
+let spot_chunked_major_alloc_shape_alloc_list_head_split
+  (mh: MH.major_heap) (fp: U64.t) (fuel: nat)
+  (requests: list nat)
+  : Lemma
+      (requires fuel > 1 /\
+                fp <> 0UL /\
+                GenInv.chunked_major_alloc_shape mh fp fuel /\
+                SpecMajorAllocMultiAlloc.all_requests_positive requests /\
+                SpecMajorAlloc.major_fl_head_wosize mh fp >=
+                  SpecMajorAllocMultiAlloc.allocation_list_demand requests + 1)
+      (ensures
+        (let r =
+           SpecMajorAllocMultiAlloc.major_alloc_list_spec
+             mh fp fuel requests in
+         r.list_fp_out <> 0UL /\
+         GenInv.chunked_major_alloc_shape r.list_major_out r.list_fp_out fuel /\
+         SpecMajorAlloc.major_fl_head_wosize
+           r.list_major_out r.list_fp_out >= 1 /\
+         SpecMajorAllocMultiAlloc.allocated_objects_nonzero
+           r.list_objs_out))
+  = GenInv.chunked_major_alloc_shape_alloc_list_head_split
+      mh fp fuel requests
 
 let spot_chunked_is_blue_preserved_by_expansion
   (mh: MH.major_heap) (fresh: MH.heap_chunk) (fp: U64.t)
